theories/Typing.v
@@ -1,0 +1,106 @@
+Require Import ssreflect.
+Require Export Arith.
+Require Export Compare_dec.
+Require Export Relations.
+Require Import ssrnat ssrfun ssrbool eqtype seq choice.
+Require Import Utf8.
+Set Implicit Arguments.
+Unset Strict Implicit.
+Unset Printing Implicit Defensive.
+
+Require Import TermEvar.
+
+Arguments fst {A B} _.
+Notation type := term.
+
+(** Typing local context *) 
+Definition ctx := list type.
+
+Definition evar_context := list (ident * (option term * type)).
+
+Inductive evar_decl : Set := 
+  { evar_ctx : evar_context;
+    evar_body : option term;
+    evar_concl : type }.
+
+Definition evar_map : Set :=
+  nat -> option evar_decl.
+
+
+Fixpoint closedn (n : nat) (t : term) : bool := 
+  match t with
+    | Srt s => true
+    | Bnd n' => n' < n
+    | Ref i => true
+    | Op b t u => closedn n t && closedn (is_abs b + 1) u
+    | Evar k l => all (closedn n) l
+  end.
+
+Definition closed := closedn 0.
+
+Fixpoint fvs (t : term) : list ident :=
+  match t with
+    | Srt s => [::]
+    | Bnd n' => [::]
+    | Ref i => [:: i]
+    | Op b t u => fvs t ++ fvs u
+    | Evar k l => flatten (map fvs l)
+  end.
+
+Definition ctx_fvs (ctx : evar_context) := map fst ctx.
+
+Fixpoint fevs (t : term) : list nat :=
+  match t with
+    | Srt s => [::]
+    | Bnd n' => [::]
+    | Ref i => [::]
+    | Op b t u => fevs t ++ fevs u
+    | Evar k l => k :: flatten (map fevs l)
+  end.
+
+Definition ctx_fevs (ctx : evar_context) := foldr (λ x acc, 
+            let: (id, (b, ty)) := x in
+              acc ++ oapp fevs [::] b ++ fevs ty) [::] ctx.
+
+Definition evar_decl_fevs evd :=
+  ctx_fevs evd.(evar_ctx) ++ 
+  fevs evd.(evar_concl) ++
+  oapp fevs [::] evd.(evar_body).
+
+Definition evar_map_fevs (e : evar_map) : list nat := [::].
+
+Definition wf_term (t : term) := 
+  closed t.
+
+Definition incl {A : eqType} (l l' : seq A) := 
+  all (λ x, x \in l') l.
+
+Definition wf_open_term (ctx : evar_context) (t : term) :=
+  incl (fvs t) (ctx_fvs ctx).
+
+Definition owf_open_term (ctx : evar_context) (b : option term) :=
+  oapp (wf_open_term ctx) true b.
+
+Definition wf_evar_context (ctx : evar_context) := 
+  let: (wfctx, b) := 
+     foldr (λ x acc, 
+            let: (wfctx, wf) := acc in
+            let: (id, (b, ty)) := x in
+              (x :: wfctx, wf && wf_open_term wfctx ty &&
+                              owf_open_term wfctx b))
+           ([::], true) ctx
+  in b.
+
+Definition wf_evar_decl evd :=
+  let ctx := evd.(evar_ctx) in
+  wf_evar_context ctx &&
+  owf_open_term ctx evd.(evar_body) &&
+  wf_open_term ctx evd.(evar_concl).
+
+Definition wf_evar_map (m : evar_map) :=
+  let mfevs := evar_map_fevs m in
+  forall k, if m k is Some x then 
+              wf_evar_decl x && incl (evar_decl_fevs x) mfevs
+            else false.
+
+                                    
