README.md
@@ -2,3 +2,16 @@ Coq-unif
 ========
 
 Formalization of unification in Coq
+
+To compile, create a symbolic link to your distribution
+of ssreflect like this:
+
+# ln -s /path/to/ssr/ ssreflect
+
+Then:
+
+# coq_makefile -f Make -o Makefile
+
+Or directly:
+
+# make
